\documentclass[a4paper,10pt]{article}
\usepackage[utf8]{inputenc}
\usepackage{geometry}

%opening
\geometry{
  body={6.5in, 9.0in},
  left=0.8in,
  top=1.0in
}

\begin{document}

%\maketitle

%\begin{abstract}

%\end{abstract}
%\section{Introduction}
The mean-field contribution to the energy-momentum tensor,
\begin{eqnarray}
T_{\kappa}^{\mu\nu}=&& \kappa(\rho\partial_{\sigma} \rho)\bigg\{\langle\partial^{\mu}u^{\sigma}\rangle u^{\nu}+\langle\partial^{\nu}u^{\sigma}\rangle u^{\mu}\bigg\} 
              +\kappa\langle\partial^{\mu}\rho\rangle \langle\partial^{\nu}\rho\rangle
              -\frac{\kappa}{2}\rho^3 \bigg\{u^{\mu}\partial^{\nu}\bigg[\frac{\vec{\nabla}\cdot \vec{v}}{\rho}\bigg]+u^{\nu}\partial^{\mu}\bigg[\frac{\vec{\nabla}\cdot \vec{v}}{\rho}\bigg] \bigg\}  \nonumber\\
              +&& \kappa\bigg\{ \frac{2}{3}\rho^{1/2}\partial^2(\rho^{3/2})-\frac{1}{2}\rho^2(\vec{\nabla}\cdot \vec{v})^2+\rho^2 u^{\alpha}\partial_{\alpha}\partial_{\beta}u^{\beta} \bigg\}g^{\mu\nu}~\nonumber\\
              -&& \kappa\bigg\{ \frac{2}{3}\rho^{1/2}\partial^2(\rho^{3/2})-\frac{3}{2}\rho^2(\vec{\nabla}\cdot \vec{v})^2 \bigg\}u^{\mu}u^{\nu}~,
\label{Eq1}              
\end{eqnarray}
with
\begin{equation}
 u^{\mu}=\gamma (1,\vec{v})~,~~~~~~~~~\gamma=\frac{1}{\sqrt{1-v^2}}~
\end{equation}
The rank-2 symmetric projection tensor is
\begin{equation}
 \langle A^{\mu}B^{\nu}\rangle=\frac{1}{2}\big\{\Delta^{\mu\alpha}\Delta^{\nu\beta}+\Delta^{\mu\beta}\Delta^{\nu\alpha}\big\}A_{\alpha}B_{\beta},~~~~~~~~\Delta^{\mu\nu}=g^{\mu\nu}-u^{\mu}u^{\nu}.
 \label{proj}
\end{equation}
For a comoving frame $u^{\mu}=(1,\vec{0})$, the property of projection tensor,
\begin{equation}
 \langle A^{0}B^{\mu}\rangle=\langle A^{\mu}B^{0}\rangle=0,
\end{equation}
since $\Delta^{\mu 0}=0$. So the projection tensor in the first two terms of $T_{\kappa}^{\mu\nu}$ only project out the vector component of the associated quantities.

The conservation equation of density $\rho$,
\begin{equation}
 D\rho=-\rho \vec{\nabla}\cdot\vec{v}~.
 \label{rho}
\end{equation}


Using these properties, from Eq.(\ref{Eq1}),

\begin{eqnarray}
 T_{\kappa}^{00}=&&0,\\
 T_{\kappa}^{ij}=&&\kappa(\partial^i \rho)(\partial^j \rho)-\kappa\big\{\rho\nabla^2\rho+\frac{1}{2}(\vec{\nabla}\rho)^2\big\}\delta^{ij}~,\\
 T_{\kappa}^{i0}=&&-\frac{\kappa}{2}(\rho\partial_j\rho)\big\{\partial^{i}u^j+\partial^j u^{i}\big\}+\frac{\kappa}{2}(\vec{\nabla}\cdot\vec{v})\big\{\rho\partial^{i}\rho\big\}-\frac{\kappa}{2}\rho^2\big\{\partial^i(\vec{\nabla}\cdot\vec{v})\big\}~.
\end{eqnarray}
Furthermore, the additional contribution to the energy density due to (\ref{Eq1}),
\begin{equation}
 u_{\mu}u_{\nu}T_{\kappa}^{\mu\nu}=0~.
\end{equation}
\\
{\bf{Important identities :}}
\begin{enumerate}
 
\item 
\begin{eqnarray}
 \nabla^2\rho=&&\nabla_{\mu}\nabla^{\mu}\rho~\nonumber\\
             =&&\partial^2\rho-D^2\rho+\frac{1}{\rho}(D\rho)^2~\nonumber\\
             =&& \partial^2\rho-D^2\rho+\rho(\vec{\nabla}\cdot \vec{v})^2~.
\label{ID1}             
\end{eqnarray}
Here, $\partial^2=\partial^{\mu}\partial_{\mu}$, $\partial_{\mu}=u_{\mu}D+\nabla_{\mu}$, $D=u^{\mu}\partial_{\mu}$ and $\nabla_{\mu}=\Delta_{\mu\nu}\partial^{\nu}$.
\\
\item
\begin{equation}
(\vec{\nabla}\rho)^2=(\nabla_{\mu}\rho)(\nabla^{\mu}\rho)=(\partial \rho)^2-(D\rho)^2~,~~~~~~~~~~~~~~~~(\partial \rho)^2=(\partial^{\mu}\rho)(\partial_{\mu}\rho)~.
\label{ID2}
\end{equation}
\\
\item With the help of Eq.(\ref{ID1}), (\ref{ID2}) and (\ref{rho}) we obtain the coefficient of the $g^{\mu\nu}$ term in Eq.(\ref{Eq1}),
\begin{eqnarray}
 \rho\nabla^2\rho+\frac{1}{2}(\vec{\nabla}\rho)^2=&&\rho\partial^2\rho+\frac{1}{2}(\partial \rho)^2-\rho D^2\rho +\frac{1}{2}(D\rho)^2\nonumber\\
 =&& \frac{2}{3}\rho^{1/2}\partial^2(\rho^{3/2})-\frac{1}{2}\rho^2(\vec{\nabla}\cdot \vec{v})^2+\rho^2 u^{\alpha}\partial_{\alpha}\partial_{\beta}u^{\beta}~,
\end{eqnarray}
where $\frac{2}{3}\rho^{1/2}\partial^2(\rho^{3/2})=\rho\partial^2\rho+\frac{1}{2}(\partial\rho)^2$ and in a comoving frame $u^{\alpha}\partial_{\alpha}\partial_{\beta}u^{\beta}=D(\vec{\nabla}\cdot\vec{v})$.
\\
\item Similarly, the coefficient of the $u^{\mu}u^{\nu}$ term in Eq.(\ref{Eq1}) turns out to be,
\begin{equation}
 \rho D^2\rho-2(D\rho)^2+\rho\nabla^2\rho+\frac{1}{2}(\vec{\nabla}\rho)^2=\frac{2}{3}\rho^{1/2}\partial^2(\rho^{3/2})-\frac{3}{2}\rho^2(\vec{\nabla}\cdot \vec{v})^2~.
\end{equation}

\end{enumerate}
\end{document}